feat: implement remaining axioms for `SingleSorted2CategoryFamily`
This implementation required the definition of some auxiliary results as
well as additional notation.

The trivial instance of `SingleSorted2Category` on the `Unit` type has
also been implemented.

Some line breaks have been improved.

InfinityCategories/HigherCategoryTheory/SingleSortedCategory/Basic.lean
@@ -4,6 +4,7 @@ Released under Apache 2.0 license as described in the file LICENSE.
 Authors: Enric Cosme Llópez, Raul Ruiz Mora, Mario Vago Marzal
 -/
 import Mathlib.Data.Pfun
+import Mathlib.Data.Part
 import InfinityCategories.Data.NatIndex
 
 /-!
@@ -14,18 +15,16 @@ universe u
 
 namespace HigherCategoryTheory
 
-class SingleSortedStruct (Obj : Type u)
-    (index : Type) [NatIndex index] where
+class SingleSortedStruct (Obj : Type u) (index : Type) [NatIndex index] where
   Sc : index → Obj → Obj
   Tg : index → Obj → Obj
   PComp : index → Obj → Obj →. Obj
   pcomp_dom : ∀ {i : index} {f g : Obj},
     (PComp i g f).Dom ↔ Sc i g = Tg i f
 
-instance {Obj : Type u}
-    {index : Type} [NatIndex index]
-    [S : SingleSortedStruct Obj index] {k : index} :
-    SingleSortedStruct Obj (Fin k) where
+instance {Obj : Type u} {index : Type} [NatIndex index]
+    [S : SingleSortedStruct Obj index]
+    {k : index} : SingleSortedStruct Obj (Fin k) where
   Sc j := S.Sc (j : index)
   Tg j := S.Tg (j : index)
   PComp j := S.PComp (j : index)
@@ -33,24 +32,38 @@ instance {Obj : Type u}
 
 scoped prefix:max "sc " => SingleSortedStruct.Sc
 scoped prefix:max "tg " => SingleSortedStruct.Tg
+scoped notation g " ♯.[" i "] " f:100 => SingleSortedStruct.PComp i g f
 
-def sc_is_tg {Obj : Type u}
-    {index : Type} [NatIndex index]
+def sc_is_tg {Obj : Type u} {index : Type} [NatIndex index]
     [SingleSortedStruct Obj index]
     (i : index) (g f : Obj) : Prop :=
   sc i g = tg i f
 
-def comp {Obj : Type u}
-    {index : Type} [NatIndex index]
-    [S : SingleSortedStruct Obj index]
+def get_dom_of_sc_is_tg {Obj : Type u} {index : Type} [NatIndex index]
+    [SingleSortedStruct Obj index]
+    {i : index} {f g : Obj} (comp_gf : sc_is_tg i g f) :
+    (g ♯.[i] f).Dom :=
+  SingleSortedStruct.pcomp_dom.mpr comp_gf
+
+def comp {Obj : Type u} {index : Type} [NatIndex index]
+    [SingleSortedStruct Obj index]
     (i : index) (g f : Obj) (composable_gf : sc_is_tg i g f) : Obj :=
-  (S.PComp i g f).get (S.pcomp_dom.mpr composable_gf)
+  (g ♯.[i] f).get (get_dom_of_sc_is_tg composable_gf)
 
-scoped notation g " ♯[" i "] " f " ← " composable_gf:100 =>
-  comp i g f composable_gf
+scoped notation g " ♯[" i "] " f " ← " comp_gf:100 => comp i g f comp_gf
 
-class SingleSortedCategoryFamily (Obj : Type u)
-    (index : Type) [NatIndex index]
+theorem congr_pcomp {Obj : Type u} {index : Type} [NatIndex index]
+    [S : SingleSortedStruct Obj index]
+    {i : index} {f₁ f₂ g₁ g₂ : Obj} (eq_g₁g₂ : g₁ = g₂) (eq_f₁f₂ : f₁ = f₂)
+    (comp_g₁f₁ : sc_is_tg i g₁ f₁) (comp_g₂f₂ : sc_is_tg i g₂ f₂) :
+    g₁ ♯[i] f₁ ← comp_g₁f₁ = g₂ ♯[i] f₂ ← comp_g₂f₂ := by
+  have pcomp_eq : g₁ ♯.[i] f₁ = g₂ ♯.[i] f₂ :=
+    congrArg₂ (· ♯.[i] ·) eq_g₁g₂ eq_f₁f₂
+  let comp_g₁f₁_dom := get_dom_of_sc_is_tg comp_g₁f₁
+  let comp_g₂f₂_dom := get_dom_of_sc_is_tg comp_g₂f₂
+  apply (Part.eq_iff_of_dom comp_g₁f₁_dom comp_g₂f₂_dom).mpr pcomp_eq
+
+class SingleSortedCategoryFamily (Obj : Type u) (index : Type) [NatIndex index]
     extends SingleSortedStruct Obj index where
   sc_sc_is_sc : ∀ {i : index} {f : Obj}, sc i (sc i f) = sc i f := by intros; rfl
   tg_sc_is_sc : ∀ {i : index} {f : Obj}, tg i (sc i f) = sc i f := by intros; rfl
@@ -72,27 +85,61 @@ class SingleSortedCategoryFamily (Obj : Type u)
     (sc_comp_is_sc comp_hg).trans comp_gf
   assoc : ∀ {i : index} {f g h : Obj} (comp_gf : sc_is_tg i g f) (comp_hg : sc_is_tg i h g),
       (h ♯[i] (g ♯[i] f ← comp_gf) ← (compr_assoc comp_gf comp_hg)) =
-      ((h ♯[i] g ← comp_hg) ♯[i] f ← (compl_assoc comp_gf comp_hg)) := by intros; rfl
+      ((h ♯[i] g ← comp_hg) ♯[i] f ← (compl_assoc comp_gf comp_hg)) := by
+      intros; rfl
 
 class SingleSorted2CategoryFamily (Obj : Type u)
     (index : Type) [NatIndex index]
     extends SingleSortedCategoryFamily Obj index where
-  sck_scj_is_scj : ∀ {k : index} {j : Fin k} {f : Obj}, sc k (sc j f) = sc j f
-  scj_is_scj_sck : ∀ {k : index} {j : Fin k} {f : Obj}, sc j f = sc j (sc k f)
-  scj_sck_is_scj_tgk : ∀ {k : index} {j : Fin k} {f : Obj}, sc j (sc k f) = sc j (tg k f)
-  tgk_tgj_is_tgj : ∀ {k : index} {j : Fin k} {f : Obj}, tg k (tg j f) = tg j f
-  tgj_is_tgj_tgk : ∀ {k : index} {j : Fin k} {f : Obj}, tg j f = tg j (tg k f)
-  tgj_tgk_is_tgj_sck : ∀ {k : index} {j : Fin k} {f : Obj}, tg j (tg k f) = tg j (sc k f)
-  sck_comp_is_comp_sck : ∀ {k : index} {j : Fin k} {f g : Obj}
+  sck_scj_is_scj : ∀ {k : index} {j : Fin k} {f : Obj}, sc k (sc j f) = sc j f := by intros; rfl
+  scj_sck_is_scj : ∀ {k : index} {j : Fin k} {f : Obj}, sc j (sc k f) = sc j f := by intros; rfl
+  scj_tgk_is_scj : ∀ {k : index} {j : Fin k} {f : Obj}, sc j (tg k f) = sc j f := by intros; rfl
+  tgk_tgj_is_tgj : ∀ {k : index} {j : Fin k} {f : Obj}, tg k (tg j f) = tg j f := by intros; rfl
+  tgj_tgk_is_tgj : ∀ {k : index} {j : Fin k} {f : Obj}, tg j (tg k f) = tg j f := by intros; rfl
+  tgj_sck_is_tgj : ∀ {k : index} {j : Fin k} {f : Obj}, tg j (sc k f) = tg j f := by intros; rfl
+  comp_j_sc {k : index} {j : Fin k} {f g : Obj} (comp_j_gf : sc_is_tg j g f) :
+      sc_is_tg j (sc k g) (sc k f) :=
+    (scj_sck_is_scj.trans comp_j_gf).trans tgj_sck_is_tgj.symm
+  comp_j_tg {k : index} {j : Fin k} {f g : Obj} (comp_j_gf : sc_is_tg j g f) :
+      sc_is_tg j (tg k g) (tg k f) :=
+    (scj_tgk_is_scj.trans comp_j_gf).trans tgj_tgk_is_tgj.symm
+  sck_compj_is_compj_sck : ∀ {k : index} {j : Fin k} {f g : Obj}
       (comp_j_gf : sc_is_tg j g f),
       sc k (g ♯[j] f ← comp_j_gf) =
-      (sc k g) ♯[j] (sc k f) ← (by sorry)
-  tgk_comp_is_comp_tgk : ∀ {k : index} {j : Fin k} {f g : Obj}
+      (sc k g) ♯[j] (sc k f) ← (comp_j_sc comp_j_gf) := by intros; rfl
+  tgk_compj_is_compj_tgk : ∀ {k : index} {j : Fin k} {f g : Obj}
       (comp_j_gf : sc_is_tg j g f),
       tg k (g ♯[j] f ← comp_j_gf) =
-      (tg k g) ♯[j] (tg k f) ← (by sorry)
-  -- TODO: Implement the remaining axiom of single-sorted 2-categories. It may
-  -- require some auxiliary axioms/definitions.
+      (tg k g) ♯[j] (tg k f) ← (comp_j_tg comp_j_gf) := by intros; rfl
+  comp_k_exchange {k : index} {j : Fin k} {f₁ f₂ g₁ g₂ : Obj}
+      (comp_k_g₂g₁ : sc_is_tg k g₂ g₁) (comp_k_f₂f₁ : sc_is_tg k f₂ f₁)
+      (comp_j_g₂f₂ : sc_is_tg j g₂ f₂) (comp_j_g₁f₁ : sc_is_tg j g₁ f₁) :
+      sc_is_tg k (g₂ ♯[j] f₂ ← comp_j_g₂f₂) (g₁ ♯[j] f₁ ← comp_j_g₁f₁) := calc
+    sc k (g₂ ♯[j] f₂ ← comp_j_g₂f₂)
+    _ = (sc k g₂) ♯[j] (sc k f₂) ← (comp_j_sc comp_j_g₂f₂) := sck_compj_is_compj_sck comp_j_g₂f₂
+    _ = (tg k g₁) ♯[j] (tg k f₁) ← (comp_j_tg comp_j_g₁f₁) :=
+      congr_pcomp comp_k_g₂g₁ comp_k_f₂f₁ (comp_j_sc comp_j_g₂f₂) (comp_j_tg comp_j_g₁f₁)
+    _ = tg k (g₁ ♯[j] f₁ ← comp_j_g₁f₁) := (tgk_compj_is_compj_tgk comp_j_g₁f₁).symm
+  comp_j_exchange {k : index} {j : Fin k} {f₁ f₂ g₁ g₂ : Obj}
+      (comp_k_g₂g₁ : sc_is_tg k g₂ g₁) (comp_k_f₂f₁ : sc_is_tg k f₂ f₁)
+      (comp_j_g₂f₂ : sc_is_tg j g₂ f₂) (comp_j_g₁f₁ : sc_is_tg j g₁ f₁) :
+      sc_is_tg j (g₂ ♯[k] g₁ ← comp_k_g₂g₁) (f₂ ♯[k] f₁ ← comp_k_f₂f₁) := calc
+    sc j (g₂ ♯[k] g₁ ← comp_k_g₂g₁)
+    _ = sc j (sc k (g₂ ♯[k] g₁ ← comp_k_g₂g₁)) := scj_sck_is_scj.symm
+    _ = sc j (sc k g₁) := congrArg (fun x => sc j x) (sc_comp_is_sc comp_k_g₂g₁)
+    _ = sc j g₁ := scj_sck_is_scj
+    _ = tg j f₁ := comp_j_g₁f₁
+    _ = tg j (sc k f₁) := tgj_sck_is_tgj.symm
+    _ = tg j (sc k (f₂ ♯[k] f₁ ← comp_k_f₂f₁)) :=
+      congrArg (fun x => tg j x) (sc_comp_is_sc comp_k_f₂f₁).symm
+    _ = tg j (f₂ ♯[k] f₁ ← comp_k_f₂f₁) := tgj_sck_is_tgj
+  exchange : ∀ {k : index} {j : Fin k} {f₁ f₂ g₁ g₂ : Obj}
+      (comp_k_g₂g₁ : sc_is_tg k g₂ g₁) (comp_k_f₂f₁ : sc_is_tg k f₂ f₁)
+      (comp_j_g₂f₂ : sc_is_tg j g₂ f₂) (comp_j_g₁f₁ : sc_is_tg j g₁ f₁),
+      (g₂ ♯[j] f₂ ← comp_j_g₂f₂) ♯[k] (g₁ ♯[j] f₁ ← comp_j_g₁f₁) ←
+        (comp_k_exchange comp_k_g₂g₁ comp_k_f₂f₁ comp_j_g₂f₂ comp_j_g₁f₁) =
+      (g₂ ♯[k] g₁ ← comp_k_g₂g₁) ♯[j] (f₂ ♯[k] f₁ ← comp_k_f₂f₁) ←
+        (comp_j_exchange comp_k_g₂g₁ comp_k_f₂f₁ comp_j_g₂f₂ comp_j_g₁f₁) := by intros; rfl
 
 @[ext]
 class SingleSortedCategory (Obj : Type u)
